fmi/fmi_export.thy
@@ -4,11 +4,440 @@
 (* Authors: Frank Zeyda and Simon Foster (University of York, UK)             *)
 (* Emails: frank.zeyda@york.ac.uk and simon.foster@york.ac.uk                 *)
 (******************************************************************************)
-(* LAST REVIEWED: 8 Feb 2017 *)
+(* LAST REVIEWED: 18 Sep 2017 *)
 
 section {* FMI {\Circus} Model *}
 
 theory fmi_export
 imports fmi
-begin
+  "../theories/utp_circus_prefix"
+begin recall_syntax
+
+declare [[syntax_ambiguity_warning = false]]
+
+subsection {* Preliminaries *}
+
+text {* The below cause ambiguities wrt their CSP definitions. *}
+
+hide_const utp_cml.Skip
+hide_const utp_cml.Stop
+
+(*
+text {* I believe the following adjustments are not required anymore. *}
+
+syntax
+  "_csp_sync" :: "logic \<Rightarrow> logic \<Rightarrow> logic" ("_ \<rightarrow>\<^sub>u _" [81, 80] 80)
+*)
+
+text {* Undeclaring Simon's prefix notation (need to parse \<open>Interaction\<close>. *}
+
+purge_syntax
+  "_output_prefix" :: "('a, '\<sigma>) uexpr \<Rightarrow> prefix_elem'" ("!'(_')")
+  "_output_prefix" :: "('a, '\<sigma>) uexpr \<Rightarrow> prefix_elem'" (".'(_')")
+
+subsection {* Lists as Tables *}
+
+type_synonym ('a, 'b) table = "('a \<times> 'b) list"
+
+fun lookup :: "('a \<times> 'b) list \<Rightarrow> 'a \<Rightarrow> 'b" where
+"lookup ((x, y) # t) v = (if v = x then y else (lookup t x))" |
+"lookup [] x = undefined"
+
+syntax "_ulookup" ::
+  "('a \<times> 'b, '\<sigma>) uexpr \<Rightarrow> ('a, '\<sigma>) uexpr \<Rightarrow> ('b, '\<sigma>) uexpr" ("lookup\<^sub>u")
+
+translations "lookup\<^sub>u t x" \<rightleftharpoons> "(CONST bop) (CONST lookup) t x"
+
+subsection {* Instantiations *}
+
+text {*
+  The instantiations below are unsafe since the type @{typ uval} may actually
+  have a higher cardinality than the continuum, depending on what HOL types we
+  inject into it! This is why I decided to adopt a shallow state model for the
+  \<open>Interaction\<close> process. (An alternative would be to adopt an axiomatic model,
+  which requires some remaining more work on integrating axiomatic variables.)
+  Strictly speaking, axiomatic values are probably not needed since the only
+  types that FMI 2.0 allows to be exchanged between FMUs are Real, Integer,
+  String and Boolean, all of which can be injected into the deep model, too.
+*}
+
+instance uval     ::        "{continuum, two}" sorry
+instance uvar_ext :: (type) "{continuum, two}" sorry
+
+subsection {* {\Circus} Constructs *}
+
+syntax "_if_then_else" ::
+  "'a upred \<Rightarrow> ('a, 'b) rel \<Rightarrow> ('a, 'b) rel \<Rightarrow> ('a, 'b) rel"
+    ("(if\<^sub>\<C> (_)/ then\<^sub>\<C> (_)/ else\<^sub>\<C> (_))" [0, 0, 10] 10)
+
+translations "if\<^sub>\<C> b then\<^sub>\<C> P else\<^sub>\<C> Q" \<rightleftharpoons> "P \<triangleleft> b \<triangleright>\<^sub>r Q"
+
+subsection {* \<open>Timer\<close> Process *}
+
+text {*
+  A problem with the {\Circus} process encoding below is that, currently, it
+  is not possible to write mixed prefixes with both inputs and outputs. Hence,
+  I had to use a trick converting everything into a single input prefix. That
+  input imposes constraints so that some parts of the communication effectively
+  behave like outputs. A second issue is that, referring to page 16 of D2.2d,
+  we see that the @{text AllowGetsAndSets} action is actually parametric. My
+  translation currently does not support parametric actions; hence I adopted
+  a solution that encodes procedure parameters by local variables. Due to the
+  proper treatment of scope by Isabelle/UTP, we generally get away with this.
+  Both issues can thus be overcome; an integration of syntax translations that
+  conceal the manual adjustments done below is pending work.
+*}
+
+text {* \todo{Write the same process as below with axiomatic variables.} *}
+
+definition
+"process TimerOld1(ct::TIME('\<tau>), hc::NZTIME('\<tau>), tN::TIME('\<tau>)) \<triangleq> begin
+  state(vstore)
+  Step =
+    (tm:setT?(t : \<guillemotleft>t \<le> tN\<guillemotright>) \<rightarrow>\<^sub>\<C> (<currentTime> := \<guillemotleft>t\<guillemotright>) ;; Step) \<box>
+    (tm:updateSS?(ss : true) \<rightarrow>\<^sub>\<C> (<stepSize> := \<guillemotleft>ss\<guillemotright>) ;; Step) \<box>
+    (tm:step![out]((&<currentTime>, &<stepSize>)\<^sub>u) \<rightarrow>\<^sub>\<C>
+      (<currentTime::'\<tau>> :=
+        min\<^sub>u(&<currentTime> + \<section>(&<stepSize::'\<tau> pos>), \<guillemotleft>tN\<guillemotright>)) ;; Step) \<box>
+    ((&<currentTime> =\<^sub>u \<guillemotleft>tN\<guillemotright>) &\<^sub>u tm:endc \<rightarrow>\<^sub>\<C> Stop)
+  \<bullet> (<currentTime>, <stepSize> := \<guillemotleft>ct\<guillemotright>, \<guillemotleft>hc\<guillemotright>) ;; Step
+end"
+
+definition
+"process TimerOld2(ct::TIME('\<tau>), hc::NZTIME('\<tau>), tN::TIME('\<tau>)) \<triangleq> begin
+  state(vstore)
+  Step =
+    (tm:setT?(t : \<guillemotleft>t \<le> tN\<guillemotright>) \<rightarrow>\<^sub>\<C> (<currentTime> := \<guillemotleft>t\<guillemotright>) ;; Step) \<box>
+    (tm:updateSS?(ss) \<rightarrow>\<^sub>\<C> (<stepSize> := \<guillemotleft>ss\<guillemotright>) ;; Step) \<box>
+    (tm:step![out\<^sub>1]($<currentTime>)![out\<^sub>2]($<stepSize>) \<rightarrow>\<^sub>\<C>
+      (<currentTime::'\<tau>> :=
+        min\<^sub>u(&<currentTime> + \<section>(&<stepSize::'\<tau> pos>), \<guillemotleft>tN\<guillemotright>)) ;; Step) \<box>
+    ((&<currentTime> =\<^sub>u \<guillemotleft>tN\<guillemotright>) &\<^sub>u tm:endc \<rightarrow>\<^sub>\<C> Stop)
+  \<bullet> (<currentTime>, <stepSize> := \<guillemotleft>ct\<guillemotright>, \<guillemotleft>hc\<guillemotright>) ;; Step
+end"
+
+subsubsection {* \<open>Interaction\<close> Process *}
+
+text {*
+  Note that I changed the type of @{text rinps} with respect to the tentative
+  model given in the deliverable D2.2d. That is, instead of using the partial
+  function type @{typ "FMI2COMP \<rightharpoonup> (VAR \<rightharpoonup> VAL)"} for @{text rinps}, I decided
+  to use the list @{typ "((FMI2COMP \<times> VAR) \<times> VAL) list"}. This is (currently)
+  a technicality since there are issues with using function types in prefixes,
+  to do with Simon's embedding of shallow variables. Using lists circumvents
+  the issue for and ought not limit generality since we may reasonably assume
+  that the port-dependency graph is a finite relation.
+*}
+
+text {* Process State: \<open>rinps :: (port \<times> VAL) list\<close>. *}
+
+definition
+"process InteractionOld \<triangleq> begin
+  state(vstore)
+  Instantiation = (;; i : FMUs \<bullet>
+    fmi:fmi2Instantiate?\<^sub>u(i_sc : \<pi>\<^sub>1(\<guillemotleft>i_sc\<guillemotright>) =\<^sub>u \<guillemotleft>i\<guillemotright>) \<rightarrow> Skip) and
+
+  InstantiationMode =
+    (if\<^sub>\<C> \<guillemotleft>parameters = []\<guillemotright> then\<^sub>\<C>
+      (;; i : FMUs \<bullet>
+        fmi:fmi2SetUpExperiment?\<^sub>u(i_startTime_stopTimeDefined_stopTime_st :
+          \<pi>\<^sub>1(\<guillemotleft>i_startTime_stopTimeDefined_stopTime_st\<guillemotright>) =\<^sub>u \<guillemotleft>i\<guillemotright> \<and>
+          \<pi>\<^sub>1(\<pi>\<^sub>2(\<guillemotleft>i_startTime_stopTimeDefined_stopTime_st\<guillemotright>)) =\<^sub>u \<guillemotleft>startTime\<guillemotright> \<and>
+          \<pi>\<^sub>1(\<pi>\<^sub>2(\<pi>\<^sub>2(\<guillemotleft>i_startTime_stopTimeDefined_stopTime_st\<guillemotright>))) =\<^sub>u \<guillemotleft>stopTimeDefined\<guillemotright> \<and>
+          \<pi>\<^sub>1(\<pi>\<^sub>2(\<pi>\<^sub>2(\<pi>\<^sub>2(\<guillemotleft>i_startTime_stopTimeDefined_stopTime_st\<guillemotright>)))) =\<^sub>u \<guillemotleft>stopTime\<guillemotright>)
+            \<rightarrow> Skip) ;;
+      (;; i : FMUs \<bullet>
+        fmi:fmi2EnterInitializationMode?\<^sub>u(i_st : \<pi>\<^sub>1(\<guillemotleft>i_st\<guillemotright>) =\<^sub>u \<guillemotleft>i\<guillemotright>) \<rightarrow> Skip)
+    else\<^sub>\<C>
+      (;; i_x_v : parameters \<bullet>
+        fmi:fmi2Set?\<^sub>u(i_x_v_st :
+          \<pi>\<^sub>1(\<guillemotleft>i_x_v_st\<guillemotright>) =\<^sub>u \<pi>\<^sub>1(\<guillemotleft>i_x_v\<guillemotright>) \<and>
+          \<pi>\<^sub>1(\<pi>\<^sub>2(\<guillemotleft>i_x_v_st\<guillemotright>)) =\<^sub>u \<pi>\<^sub>1(\<pi>\<^sub>2(\<guillemotleft>i_x_v\<guillemotright>)) \<and>
+          \<pi>\<^sub>1(\<pi>\<^sub>2(\<pi>\<^sub>2(\<guillemotleft>i_x_v_st\<guillemotright>))) =\<^sub>u \<pi>\<^sub>2(\<pi>\<^sub>2(\<guillemotleft>i_x_v\<guillemotright>))) \<rightarrow> Skip) ;;
+      (;; i : FMUs \<bullet>
+        fmi:fmi2SetUpExperiment?\<^sub>u(i_startTime_stopTimeDefined_stopTime_st :
+          \<pi>\<^sub>1(\<guillemotleft>i_startTime_stopTimeDefined_stopTime_st\<guillemotright>) =\<^sub>u \<guillemotleft>i\<guillemotright> \<and>
+          \<pi>\<^sub>1(\<pi>\<^sub>2(\<guillemotleft>i_startTime_stopTimeDefined_stopTime_st\<guillemotright>)) =\<^sub>u \<guillemotleft>startTime\<guillemotright> \<and>
+          \<pi>\<^sub>1(\<pi>\<^sub>2(\<pi>\<^sub>2(\<guillemotleft>i_startTime_stopTimeDefined_stopTime_st\<guillemotright>))) =\<^sub>u \<guillemotleft>stopTimeDefined\<guillemotright> \<and>
+          \<pi>\<^sub>1(\<pi>\<^sub>2(\<pi>\<^sub>2(\<pi>\<^sub>2(\<guillemotleft>i_startTime_stopTimeDefined_stopTime_st\<guillemotright>)))) =\<^sub>u \<guillemotleft>stopTime\<guillemotright>)
+            \<rightarrow> Skip) ;;
+      (;; i : FMUs \<bullet>
+        fmi:fmi2EnterInitializationMode?\<^sub>u(i_st : \<pi>\<^sub>1(\<guillemotleft>i_st\<guillemotright>) =\<^sub>u \<guillemotleft>i\<guillemotright>) \<rightarrow> Skip)) and
+
+  InitializationMode =
+    (if\<^sub>\<C> \<guillemotleft>initialValues = []\<guillemotright> then\<^sub>\<C>
+      (;; i : FMUs \<bullet>
+        fmi:fmi2ExitInitializationMode?\<^sub>u(i_st : \<pi>\<^sub>1(\<guillemotleft>i_st\<guillemotright>) =\<^sub>u \<guillemotleft>i\<guillemotright>) \<rightarrow> Skip)
+    else\<^sub>\<C>
+      (;; i_x_v : initialValues \<bullet>
+        fmi:fmi2Set?\<^sub>u(i_x_v_st :
+          \<pi>\<^sub>1(\<guillemotleft>i_x_v_st\<guillemotright>) =\<^sub>u \<pi>\<^sub>1(\<guillemotleft>i_x_v\<guillemotright>) \<and>
+          \<pi>\<^sub>1(\<pi>\<^sub>2(\<guillemotleft>i_x_v_st\<guillemotright>)) =\<^sub>u \<pi>\<^sub>1(\<pi>\<^sub>2(\<guillemotleft>i_x_v\<guillemotright>)) \<and>
+          \<pi>\<^sub>1(\<pi>\<^sub>2(\<pi>\<^sub>2(\<guillemotleft>i_x_v_st\<guillemotright>))) =\<^sub>u \<pi>\<^sub>2(\<pi>\<^sub>2(\<guillemotleft>i_x_v\<guillemotright>))) \<rightarrow> Skip) ;;
+      (;; i : FMUs \<bullet>
+        fmi:fmi2ExitInitializationMode?\<^sub>u(i_st : \<pi>\<^sub>1(\<guillemotleft>i_st\<guillemotright>) =\<^sub>u \<guillemotleft>i\<guillemotright>) \<rightarrow> Skip)) and
+
+  Terminated = (;; i : FMUs \<bullet>
+    fmi:fmi2Terminate?\<^sub>u(i_st : \<pi>\<^sub>1(\<guillemotleft>i_st\<guillemotright>) =\<^sub>u \<guillemotleft>i\<guillemotright>) \<rightarrow>
+    fmi:fmi2FreeInstance?\<^sub>u(i_st : \<pi>\<^sub>1(\<guillemotleft>i_st\<guillemotright>) =\<^sub>u \<guillemotleft>i\<guillemotright>) \<rightarrow> Skip) ;;
+    ctr:endsimulation \<rightarrow>\<^sub>u Skip and
+
+  TakeOutputs = <rinp::(port \<times> VAL) list> := \<langle>\<rangle> ;;
+    (;; out : outputs \<bullet> fmi:fmi2Get?\<^sub>u(i_x_v_st :
+      \<pi>\<^sub>1(\<guillemotleft>i_x_v_st\<guillemotright>) =\<^sub>u \<guillemotleft>FMU out\<guillemotright> \<and>
+      \<pi>\<^sub>1(\<pi>\<^sub>2(\<guillemotleft>i_x_v_st\<guillemotright>)) =\<^sub>u \<guillemotleft>name out\<guillemotright>) \<rightarrow>
+        (;; inp : pdg out \<bullet>
+          <rinp> := &<rinp> ^\<^sub>u \<langle>(\<guillemotleft>inp\<guillemotright>, \<pi>\<^sub>1(\<pi>\<^sub>2(\<pi>\<^sub>2(&i_x_v_st))))\<^sub>u\<rangle>)) and
+
+  DistributeInputs = (;; inp : inputs \<bullet>
+    fmi:fmi2Set?\<^sub>u(i_x_v_st :
+      \<pi>\<^sub>1(\<guillemotleft>i_x_v_st\<guillemotright>) =\<^sub>u \<guillemotleft>FMU inp\<guillemotright> \<and>
+      \<pi>\<^sub>1(\<pi>\<^sub>2(\<guillemotleft>i_x_v_st\<guillemotright>)) =\<^sub>u \<guillemotleft>name inp\<guillemotright> \<and>
+      \<pi>\<^sub>1(\<pi>\<^sub>2(\<pi>\<^sub>2(\<guillemotleft>i_x_v_st\<guillemotright>))) =\<^sub>u (lookup\<^sub>u $<rinp> \<guillemotleft>inp\<guillemotright>)) \<rightarrow> Skip) and
+
+  Step = (;; i : [0..(length FMUs)] \<bullet>
+    (if (i::int) = 0 then
+      ctr:stepToComplete \<rightarrow>\<^sub>u
+        (fmi:fmi2DoStep?\<^sub>u(i_t_hc_st :
+          \<pi>\<^sub>1(\<guillemotleft>i_t_hc_st\<guillemotright>) =\<^sub>u \<guillemotleft>nth FMUs 1\<guillemotright> \<and>
+          \<pi>\<^sub>1(\<pi>\<^sub>2(\<guillemotleft>i_t_hc_st\<guillemotright>)) =\<^sub>u $<t> \<and>
+          \<pi>\<^sub>1(\<pi>\<^sub>2(\<pi>\<^sub>2(\<guillemotleft>i_t_hc_st\<guillemotright>))) =\<^sub>u $<hc>) \<rightarrow> Skip)
+    else if (i::int) < (length FMUs) then
+      (\<mu> X \<bullet>
+        (fmi:fmi2GetBooleanStatusfmi2Terminated?\<^sub>u(i_b_st :
+          \<pi>\<^sub>1(\<guillemotleft>i_b_st\<guillemotright>) =\<^sub>u \<guillemotleft>nth FMUs (nat i)\<guillemotright>) \<rightarrow> X) \<box>
+        (fmi:fmi2GetMaxStepSize?\<^sub>u(i_t_st :
+          \<pi>\<^sub>1(\<guillemotleft>i_t_st\<guillemotright>) =\<^sub>u \<guillemotleft>nth FMUs (nat i)\<guillemotright>) \<rightarrow> X)) \<box>
+        (fmi:fmi2DoStep?\<^sub>u(i_t_hc_st :
+          \<pi>\<^sub>1(\<guillemotleft>i_t_hc_st\<guillemotright>) =\<^sub>u \<guillemotleft>nth FMUs (nat (i+1))\<guillemotright> \<and>
+          \<pi>\<^sub>1(\<pi>\<^sub>2(\<guillemotleft>i_t_hc_st\<guillemotright>)) =\<^sub>u $<t> \<and>
+          \<pi>\<^sub>1(\<pi>\<^sub>2(\<pi>\<^sub>2(\<guillemotleft>i_t_hc_st\<guillemotright>))) =\<^sub>u $<hc>) \<rightarrow> Skip)
+    else
+      (\<mu> X \<bullet>
+        (fmi:fmi2GetBooleanStatusfmi2Terminated?\<^sub>u(i_b_st :
+          \<pi>\<^sub>1(\<guillemotleft>i_b_st\<guillemotright>) =\<^sub>u \<guillemotleft>nth FMUs (nat i)\<guillemotright>) \<rightarrow> X) \<box>
+        (fmi:fmi2GetMaxStepSize?\<^sub>u(i_t_st :
+          \<pi>\<^sub>1(\<guillemotleft>i_t_st\<guillemotright>) =\<^sub>u \<guillemotleft>nth FMUs (nat i)\<guillemotright>) \<rightarrow> X)) \<box>
+        (ctr:stepAnalysed \<rightarrow>\<^sub>u Skip))) and
+
+  slaveInitialized =
+    (tm:endc \<rightarrow>\<^sub>u Terminated) \<box>
+    (tm:step?\<^sub>u(t_hc : true) \<rightarrow>
+      (* Used local variables to pass action parameters! *)
+      (<t>, <hc> := \<pi>\<^sub>1(&t_hc), \<pi>\<^sub>2(&t_hc)) ;;
+      TakeOutputs ;; DistributeInputs ;; Step) and
+
+  NextStep =
+    (tm:updateSS?\<^sub>u(d : true) \<rightarrow> NextStep) \<box>
+    (tm:setT?\<^sub>u(t : true) \<rightarrow> NextStep) \<box>
+    (slaveInitialized ;; NextStep) \<box>
+    (Terminated)
+
+  \<bullet> Instantiation ;; InstantiationMode ;; InitializationMode ;; slaveInitialized
+end"
+
+theorem "P InteractionOld"
+apply (unfold InteractionOld_def)
+apply (simp add: circus_syntax Let_def)
+oops
+
+text {* A simplified definition of the same (?) process is given below. *}
+
+definition
+"process InteractionSimplified \<triangleq> begin
+  state(vstore)
+  Instantiation = (;; i : FMUs \<bullet>
+    fmi:fmi2Instantiate?\<^sub>u(i_sc : \<pi>\<^sub>1(\<guillemotleft>i_sc\<guillemotright>) =\<^sub>u \<guillemotleft>i\<guillemotright>) \<rightarrow> Skip) and
+
+  InstantiationMode =
+    (;; i_x_v : parameters \<bullet>
+      fmi:fmi2Set?\<^sub>u(i_x_v_st :
+        \<pi>\<^sub>1(\<guillemotleft>i_x_v_st\<guillemotright>) =\<^sub>u \<pi>\<^sub>1(\<guillemotleft>i_x_v\<guillemotright>) \<and>
+        \<pi>\<^sub>1(\<pi>\<^sub>2(\<guillemotleft>i_x_v_st\<guillemotright>)) =\<^sub>u \<pi>\<^sub>1(\<pi>\<^sub>2(\<guillemotleft>i_x_v\<guillemotright>)) \<and>
+        \<pi>\<^sub>1(\<pi>\<^sub>2(\<pi>\<^sub>2(\<guillemotleft>i_x_v_st\<guillemotright>))) =\<^sub>u \<pi>\<^sub>2(\<pi>\<^sub>2(\<guillemotleft>i_x_v\<guillemotright>))) \<rightarrow> Skip) ;;
+    (;; i : FMUs \<bullet>
+      fmi:fmi2SetUpExperiment?\<^sub>u(i_startTime_stopTimeDefined_stopTime_st :
+        \<pi>\<^sub>1(\<guillemotleft>i_startTime_stopTimeDefined_stopTime_st\<guillemotright>) =\<^sub>u \<guillemotleft>i\<guillemotright> \<and>
+        \<pi>\<^sub>1(\<pi>\<^sub>2(\<guillemotleft>i_startTime_stopTimeDefined_stopTime_st\<guillemotright>)) =\<^sub>u \<guillemotleft>startTime\<guillemotright> \<and>
+        \<pi>\<^sub>1(\<pi>\<^sub>2(\<pi>\<^sub>2(\<guillemotleft>i_startTime_stopTimeDefined_stopTime_st\<guillemotright>))) =\<^sub>u \<guillemotleft>stopTimeDefined\<guillemotright> \<and>
+        \<pi>\<^sub>1(\<pi>\<^sub>2(\<pi>\<^sub>2(\<pi>\<^sub>2(\<guillemotleft>i_startTime_stopTimeDefined_stopTime_st\<guillemotright>)))) =\<^sub>u \<guillemotleft>stopTime\<guillemotright>)
+          \<rightarrow> Skip) ;;
+    (;; i : FMUs \<bullet>
+      fmi:fmi2EnterInitializationMode?\<^sub>u(i_st : \<pi>\<^sub>1(\<guillemotleft>i_st\<guillemotright>) =\<^sub>u \<guillemotleft>i\<guillemotright>) \<rightarrow> Skip) and
+
+  InitializationMode =
+    (;; i_x_v : initialValues \<bullet>
+      fmi:fmi2Set?\<^sub>u(i_x_v_st :
+        \<pi>\<^sub>1(\<guillemotleft>i_x_v_st\<guillemotright>) =\<^sub>u \<pi>\<^sub>1(\<guillemotleft>i_x_v\<guillemotright>) \<and>
+        \<pi>\<^sub>1(\<pi>\<^sub>2(\<guillemotleft>i_x_v_st\<guillemotright>)) =\<^sub>u \<pi>\<^sub>1(\<pi>\<^sub>2(\<guillemotleft>i_x_v\<guillemotright>)) \<and>
+        \<pi>\<^sub>1(\<pi>\<^sub>2(\<pi>\<^sub>2(\<guillemotleft>i_x_v_st\<guillemotright>))) =\<^sub>u \<pi>\<^sub>2(\<pi>\<^sub>2(\<guillemotleft>i_x_v\<guillemotright>))) \<rightarrow> Skip) ;;
+    (;; i : FMUs \<bullet>
+      fmi:fmi2ExitInitializationMode?\<^sub>u(i_st : \<pi>\<^sub>1(\<guillemotleft>i_st\<guillemotright>) =\<^sub>u \<guillemotleft>i\<guillemotright>) \<rightarrow> Skip) and
+
+  Terminated = (;; i : FMUs \<bullet>
+    fmi:fmi2Terminate?\<^sub>u(i_st : \<pi>\<^sub>1(\<guillemotleft>i_st\<guillemotright>) =\<^sub>u \<guillemotleft>i\<guillemotright>) \<rightarrow>
+    fmi:fmi2FreeInstance?\<^sub>u(i_st : \<pi>\<^sub>1(\<guillemotleft>i_st\<guillemotright>) =\<^sub>u \<guillemotleft>i\<guillemotright>) \<rightarrow> Skip) ;;
+    ctr:endsimulation \<rightarrow>\<^sub>u Skip and
+
+  TakeOutputs = <rinp::(port \<times> VAL) list> := \<langle>\<rangle> ;;
+    (;; out : outputs \<bullet> fmi:fmi2Get?\<^sub>u(i_x_v_st :
+      \<pi>\<^sub>1(\<guillemotleft>i_x_v_st\<guillemotright>) =\<^sub>u \<guillemotleft>FMU out\<guillemotright> \<and>
+      \<pi>\<^sub>1(\<pi>\<^sub>2(\<guillemotleft>i_x_v_st\<guillemotright>)) =\<^sub>u \<guillemotleft>name out\<guillemotright>) \<rightarrow>
+        (;; inp : pdg out \<bullet>
+          <rinp> := &<rinp> ^\<^sub>u \<langle>(\<guillemotleft>inp\<guillemotright>, \<pi>\<^sub>1(\<pi>\<^sub>2(\<pi>\<^sub>2(&i_x_v_st))))\<^sub>u\<rangle>)) and
+
+  DistributeInputs = (;; inp : inputs \<bullet>
+    fmi:fmi2Set?\<^sub>u(i_x_v_st :
+      \<pi>\<^sub>1(\<guillemotleft>i_x_v_st\<guillemotright>) =\<^sub>u \<guillemotleft>FMU inp\<guillemotright> \<and>
+      \<pi>\<^sub>1(\<pi>\<^sub>2(\<guillemotleft>i_x_v_st\<guillemotright>)) =\<^sub>u \<guillemotleft>name inp\<guillemotright> \<and>
+      \<pi>\<^sub>1(\<pi>\<^sub>2(\<pi>\<^sub>2(\<guillemotleft>i_x_v_st\<guillemotright>))) =\<^sub>u (lookup\<^sub>u $<rinp> \<guillemotleft>inp\<guillemotright>)) \<rightarrow> Skip) and
+
+  Step = (;; i : [0..(length FMUs)] \<bullet>
+    (if (i::int) = 0 then
+      ctr:stepToComplete \<rightarrow>\<^sub>u
+        (fmi:fmi2DoStep?\<^sub>u(i_t_hc_st :
+          \<pi>\<^sub>1(\<guillemotleft>i_t_hc_st\<guillemotright>) =\<^sub>u \<guillemotleft>nth FMUs 1\<guillemotright> \<and>
+          \<pi>\<^sub>1(\<pi>\<^sub>2(\<guillemotleft>i_t_hc_st\<guillemotright>)) =\<^sub>u $<t> \<and>
+          \<pi>\<^sub>1(\<pi>\<^sub>2(\<pi>\<^sub>2(\<guillemotleft>i_t_hc_st\<guillemotright>))) =\<^sub>u $<hc>) \<rightarrow> Skip)
+    else if (i::int) < (length FMUs) then
+      (\<mu> X \<bullet>
+        (fmi:fmi2GetBooleanStatusfmi2Terminated?\<^sub>u(i_b_st :
+          \<pi>\<^sub>1(\<guillemotleft>i_b_st\<guillemotright>) =\<^sub>u \<guillemotleft>nth FMUs (nat i)\<guillemotright>) \<rightarrow> X) \<box>
+        (fmi:fmi2GetMaxStepSize?\<^sub>u(i_t_st :
+          \<pi>\<^sub>1(\<guillemotleft>i_t_st\<guillemotright>) =\<^sub>u \<guillemotleft>nth FMUs (nat i)\<guillemotright>) \<rightarrow> X)) \<box>
+        (fmi:fmi2DoStep?\<^sub>u(i_t_hc_st :
+          \<pi>\<^sub>1(\<guillemotleft>i_t_hc_st\<guillemotright>) =\<^sub>u \<guillemotleft>nth FMUs (nat (i+1))\<guillemotright> \<and>
+          \<pi>\<^sub>1(\<pi>\<^sub>2(\<guillemotleft>i_t_hc_st\<guillemotright>)) =\<^sub>u $<t> \<and>
+          \<pi>\<^sub>1(\<pi>\<^sub>2(\<pi>\<^sub>2(\<guillemotleft>i_t_hc_st\<guillemotright>))) =\<^sub>u $<hc>) \<rightarrow> Skip)
+    else
+      (\<mu> X \<bullet>
+        (fmi:fmi2GetBooleanStatusfmi2Terminated?\<^sub>u(i_b_st :
+          \<pi>\<^sub>1(\<guillemotleft>i_b_st\<guillemotright>) =\<^sub>u \<guillemotleft>nth FMUs (nat i)\<guillemotright>) \<rightarrow> X) \<box>
+        (fmi:fmi2GetMaxStepSize?\<^sub>u(i_t_st :
+          \<pi>\<^sub>1(\<guillemotleft>i_t_st\<guillemotright>) =\<^sub>u \<guillemotleft>nth FMUs (nat i)\<guillemotright>) \<rightarrow> X)) \<box>
+        (ctr:stepAnalysed \<rightarrow>\<^sub>u Skip))) and
+
+  slaveInitialized =
+    (tm:endc \<rightarrow>\<^sub>u Terminated) \<box>
+    (tm:step?\<^sub>u(t_hc : true) \<rightarrow>
+      (* Used local variables to pass action parameters! *)
+      (<t>, <hc> := \<pi>\<^sub>1(&t_hc), \<pi>\<^sub>2(&t_hc)) ;;
+      TakeOutputs ;; DistributeInputs ;; Step) and
+
+  NextStep =
+    (tm:updateSS?\<^sub>u(d : true) \<rightarrow> NextStep) \<box>
+    (tm:setT?\<^sub>u(t : true) \<rightarrow> NextStep) \<box>
+    (slaveInitialized ;; NextStep) \<box>
+    (Terminated)
+
+  \<bullet> Instantiation ;; InstantiationMode ;; InitializationMode ;; slaveInitialized
+end"
+
+definition
+"process InteractionNew \<triangleq> begin
+  state(vstore)
+  Instantiation = (;; i : FMUs \<bullet>
+    fmi:fmi2Instantiate.[out\<^sub>1](\<guillemotleft>i\<guillemotright>)?(sc) \<rightarrow>\<^sub>\<C> Skip) and
+
+  InstantiationMode =
+    (;; (i, x, v) : parameters \<bullet>
+      fmi:fmi2Set![out\<^sub>1](\<guillemotleft>i\<guillemotright>)![out\<^sub>2](\<guillemotleft>x\<guillemotright>)![out\<^sub>3](\<guillemotleft>v\<guillemotright>)?(st) \<rightarrow>\<^sub>\<C> Skip) ;;
+    (;; i : FMUs \<bullet>
+      fmi:fmi2SetUpExperiment![out\<^sub>1](\<guillemotleft>i\<guillemotright>)![out\<^sub>2](\<guillemotleft>startTime\<guillemotright>)
+        ![out\<^sub>3](\<guillemotleft>stopTimeDefined\<guillemotright>)![out\<^sub>4](\<guillemotleft>stopTime\<guillemotright>)?(st) \<rightarrow>\<^sub>\<C> Skip) ;;
+    (;; i : FMUs \<bullet>
+      fmi:fmi2EnterInitializationMode.[out\<^sub>1](\<guillemotleft>i\<guillemotright>)?(sc) \<rightarrow>\<^sub>\<C> Skip) and
+
+  InitializationMode =
+    (;; (i, x, v) : initialValues \<bullet>
+      fmi:fmi2Set![out\<^sub>1](\<guillemotleft>i\<guillemotright>)![out\<^sub>2](\<guillemotleft>x\<guillemotright>)![out\<^sub>3](\<guillemotleft>v\<guillemotright>)?(st) \<rightarrow>\<^sub>\<C> Skip) ;;
+    (;; i : FMUs \<bullet>
+      fmi:fmi2ExitInitializationMode![out\<^sub>1](\<guillemotleft>i\<guillemotright>)?(sc) \<rightarrow>\<^sub>\<C> Skip) and
+
+  Terminated =
+    (;; i : FMUs \<bullet>
+      fmi:fmi2Terminate.[out\<^sub>1](\<guillemotleft>i\<guillemotright>)?(sc) \<rightarrow>\<^sub>\<C>
+      fmi:fmi2FreeInstance.[out\<^sub>1](\<guillemotleft>i\<guillemotright>)?(sc) \<rightarrow>\<^sub>\<C> Skip) ;;
+    ctr:endsimulation \<rightarrow>\<^sub>\<C> Skip and
+
+  TakeOutputs = <rinp::(port \<times> VAL) list> := \<langle>\<rangle> ;;
+    (;; out : outputs \<bullet>
+      fmi:fmi2Get.[out\<^sub>1](\<guillemotleft>FMU out\<guillemotright>).[out\<^sub>2](\<guillemotleft>name out\<guillemotright>)?(v)?(st) \<rightarrow>\<^sub>\<C>
+        (;; inp : pdg out \<bullet> <rinp> := &<rinp> ^\<^sub>u \<langle>(\<guillemotleft>inp\<guillemotright>, \<guillemotleft>v\<guillemotright>)\<^sub>u\<rangle>)) and
+
+  DistributeInputs = (;; inp : inputs \<bullet>
+    fmi:fmi2Set.[out\<^sub>1](\<guillemotleft>FMU inp\<guillemotright>).[out\<^sub>2](\<guillemotleft>name inp\<guillemotright>)
+      ![out\<^sub>3](lookup\<^sub>u $<rinp> \<guillemotleft>inp\<guillemotright>)?(st) \<rightarrow>\<^sub>\<C> Skip) and
+
+  Step = (;; i : [0..(length FMUs)] \<bullet>
+    (if (i::int) = 0 then
+      ctr:stepToComplete \<rightarrow>\<^sub>\<C>
+        (fmi:fmi2DoStep.[out\<^sub>1](\<guillemotleft>FMUs!0\<guillemotright>).[out\<^sub>2]($<t>).[out\<^sub>3]($<hc>)?(st) \<rightarrow>\<^sub>\<C> Skip)
+    else if (i::int) < (length FMUs) then
+      (\<mu> X \<bullet>
+        (fmi:fmi2GetBooleanStatusfmi2Terminated.[out\<^sub>1](\<guillemotleft>FMUs!(nat (i-1))\<guillemotright>)?(b)?(st) \<rightarrow>\<^sub>\<C> X) \<box>
+        (fmi:fmi2GetMaxStepSize.[out\<^sub>1](\<guillemotleft>FMUs!(nat (i-1))\<guillemotright>)?(t)?(st) \<rightarrow>\<^sub>\<C> X)) \<box>
+        (fmi:fmi2DoStep.[out\<^sub>1](\<guillemotleft>FMUs!(nat i)\<guillemotright>).[out\<^sub>2]($<t>).[out\<^sub>3]($<hc>)?(st) \<rightarrow>\<^sub>\<C> Skip)
+    else
+      (\<mu> X \<bullet>
+        (fmi:fmi2GetBooleanStatusfmi2Terminated.[out\<^sub>1](\<guillemotleft>FMUs!(nat (i-1))\<guillemotright>)?(b)?(st) \<rightarrow>\<^sub>\<C> X) \<box>
+        (fmi:fmi2GetMaxStepSize.[out\<^sub>1](\<guillemotleft>FMUs!(nat (i-1))\<guillemotright>)?(t)?(st) \<rightarrow>\<^sub>\<C> X)) \<box>
+        (ctr:stepAnalysed \<rightarrow>\<^sub>\<C> Skip))) and
+
+  slaveInitialized =
+    (tm:endc \<rightarrow>\<^sub>\<C> Terminated) \<box>
+    (tm:step?(t)?(hc) \<rightarrow>\<^sub>\<C>
+      (* We use local variables to pass action parameters! *)
+      (<t>, <hc> := \<guillemotleft>t\<guillemotright>, \<guillemotleft>hc\<guillemotright>) ;;
+      TakeOutputs ;; DistributeInputs ;; Step) and
+
+  NextStep =
+    (tm:updateSS?(d) \<rightarrow>\<^sub>\<C> NextStep) \<box>
+    (tm:setT?(t) \<rightarrow>\<^sub>\<C> NextStep) \<box>
+    (slaveInitialized ;; NextStep) \<box>
+    (Terminated)
+
+  \<bullet> Instantiation ;; InstantiationMode ;; InitializationMode ;; slaveInitialized
+end"
+
+theorem "P InteractionNew"
+apply (unfold InteractionNew_def)
+apply (simp add: circus_syntax Let_def)
+oops
+
+subsubsection {* \<open>FMUStatesManager\<close> Process *}
+
+definition
+"process FMUStatesManagerOld1(i::FMI2COMP) \<triangleq> begin
+  state(vstore)
+  AllowsGetsAndSets =
+    (fmi:fmi2GetFMUState?\<^sub>u(i_s_st : \<pi>\<^sub>1(\<guillemotleft>i_s_st\<guillemotright>) =\<^sub>u \<guillemotleft>i\<guillemotright>) \<rightarrow>
+      (<s> := \<pi>\<^sub>1(\<pi>\<^sub>2(&i_s_st)) ;; AllowsGetsAndSets)) \<box>
+    (fmi:fmi2SetFMUState?\<^sub>u(i_s_st : \<pi>\<^sub>1(\<guillemotleft>i_s_st\<guillemotright>) =\<^sub>u \<guillemotleft>i\<guillemotright> \<and> \<pi>\<^sub>1(\<pi>\<^sub>2(\<guillemotleft>i_s_st\<guillemotright>)) =\<^sub>u $<s>) \<rightarrow>
+      (<s> := \<pi>\<^sub>1(\<pi>\<^sub>2(&i_s_st)) ;; AllowsGetsAndSets)) and
+  AllowAGet =
+    (fmi:fmi2GetFMUState?\<^sub>u(i_s_st : \<pi>\<^sub>1(\<guillemotleft>i_s_st\<guillemotright>) =\<^sub>u \<guillemotleft>i\<guillemotright>) \<rightarrow>
+      (<s> := \<pi>\<^sub>1(\<pi>\<^sub>2(&i_s_st)) ;; AllowsGetsAndSets))
+  \<bullet> fmi:fmi2Instantiate?\<^sub>u(i_b : \<pi>\<^sub>1(\<guillemotleft>i_b\<guillemotright>) =\<^sub>u \<guillemotleft>i\<guillemotright>) \<rightarrow> AllowAGet
+end"
+
+definition
+"process FMUStatesManagerOld2(i::FMI2COMP) \<triangleq> begin
+  state(vstore)
+  AllowsGetsAndSets =
+    (fmi:fmi2GetFMUState![out](\<guillemotleft>i\<guillemotright>)?(s)?(st) \<rightarrow>\<^sub>\<C> (<s> := \<guillemotleft>s\<guillemotright>) ;; AllowsGetsAndSets) \<box>
+    (fmi:fmi2SetFMUState![out\<^sub>1](\<guillemotleft>i\<guillemotright>)![out\<^sub>2](&<s>) \<rightarrow>\<^sub>\<C> AllowsGetsAndSets) and
+  AllowAGet =
+    (fmi:fmi2GetFMUState![out](\<guillemotleft>i\<guillemotright>)?(s)?(st) \<rightarrow>\<^sub>\<C> (<s> := \<guillemotleft>s\<guillemotright>) ;; AllowsGetsAndSets)
+  \<bullet> fmi:fmi2Instantiate![out](\<guillemotleft>i\<guillemotright>)?(b) \<rightarrow>\<^sub>\<C> AllowAGet
+end"
+
+subsection {* Proof Experiments *}
+
+term "setT!\<^sub>u(\<guillemotleft>0\<guillemotright>) \<rightarrow> SKIP"
+term "InputCSP setT x"
+term "\<lceil>''x''\<rceil>\<^sub>d"
+term "(dvar_lens \<lceil>''x''\<rceil>\<^sub>d)"
+term "\<lceil>''x''\<rceil>\<^sub>d\<up>"
+term "InputCircus setT (\<lceil>''x''\<rceil>\<^sub>d\<up>)"
 end
